src/Crypto/NeqSigma.v
@@ -1,8 +1,7 @@
-(* 
 From Stdlib Require Import Setoid
   setoid_ring.Field Lia Vector Utf8
   Psatz Bool Pnat BinNatDef 
-  BinPos. 
+  BinPos Arith.
 From Algebra Require Import 
   Hierarchy Group Monoid
   Field Integral_domain
@@ -12,12 +11,117 @@ From Probability Require Import
 From Utility Require Import Util. 
 From ExtLib Require Import Monad. 
 From Crypto Require Import Sigma 
-  AndSigma.
+  AndSigmaGen Okamoto.
 
 Import MonadNotation 
   VectorNotations.
-
+          
 #[local] Open Scope monad_scope.
+
+Section Util.
+
+  (* 
+    Theorem add_zero_trans : ∀ (n : nat), n + 0 = n.
+    Admitted. 
+    
+    Theorem add_commutative : ∀ (a b : nat), a + b = b + a.
+    Admitted.
+
+    Theorem add_mul_comm : ∀ (a b : nat), a * b = b * a. 
+    Admitted. 
+
+    Theorem add_comm_dist_transparent : ∀ (a b c : nat), 
+     (a + b) * c = a * c + b * c.
+    Proof.
+    Admitted.
+      
+      
+
+    Theorem add_comm_transparent : ∀ (n : nat),
+      (1 + S n) * 2 + ((2 + n) * (1 + n)) = (2 + S n) * (1 + S n).
+    Proof.
+      intros *. change (S n) with (1 + n).
+      rewrite !add_comm_dist_transparent.
+      setoid_rewrite add_mul_comm.
+      cbn.  f_equal. f_equal.
+      f_equal. f_equal.
+      rewrite add_zero_trans.
+      rewrite add_commutative.
+      setoid_rewrite add_commutative at 1.
+      f_equal. 
+      change 2 with (1 + 1).
+      rewrite add_mul_comm, add_comm_dist_transparent.
+      cbn; rewrite !add_zero_trans; reflexivity.
+      f_equal. f_equal.
+      cbn. change 2 with (1 + 1).
+      rewrite add_mul_comm, add_comm_dist_transparent.
+      cbn; rewrite !add_zero_trans.
+      f_equal.
+  *)
+
+
+    (* computes pair of vectors: *)
+    Fixpoint generate_pairs_of_vector {A : Type} {n : nat}  
+      (gs : Vector.t A (2 + n)) : Vector.t (A * A) (Nat.div ((2 + n) * (1 + n)) 2).
+    Proof.
+      destruct n as [|n].
+      +
+        destruct (vector_inv_S gs) as (gsh & gst & _).
+        destruct (vector_inv_S gst) as (gsth & _).
+        exact [(gsh, gsth)].
+      +
+        destruct (vector_inv_S gs) as (gsh & gst & _).
+        (* map gsh over gst *)
+        set (reta := Vector.map (fun x => (gsh, x)) gst).
+        specialize (generate_pairs_of_vector _ _ gst).
+        (* make this proof transparent. *)
+        assert (ha : ((1 + S n) * 2 + ((2 + n) * (1 + n)) = 
+        ((2 + S n) * (1 + S n)))%nat) by (abstract nia).
+        eapply f_equal with (f := fun x => Nat.div x 2) in ha.
+        rewrite PeanoNat.Nat.div_add_l in ha; try (abstract nia).
+        refine(@eq_rect nat _ (Vector.t (A * A)) (reta ++ generate_pairs_of_vector) _
+          ha).
+    Defined.
+
+   
+    Definition nat_div_2 : ∀ (n : nat), 
+        (2 * Nat.div ((2 + n) * (1 + n)) 2)%nat = ((2 + n) * (1 + n))%nat.
+      Proof.
+        induction n as [| n IH].
+        - (* Base case: n = 0 *)
+          cbn; reflexivity.
+        - (* Inductive step *)
+          change ((2 + S n))%nat with (3 + n)%nat.
+          change ((1 + S n))%nat with (2 + n)%nat.
+          (* We show that (n+3)(n+2) = (n+2)(n+1) + 2(n+2) *)
+          replace ((3 + n) * (2 + n))%nat
+            with (((2 + n) * (1 + n)) + 2 * (2 + n))%nat
+            by (abstract nia).
+          replace (2 * (2 + n))%nat with 
+          ((2 + n) * 2)%nat by (abstract nia).
+          rewrite Nat.div_add; 
+          try (abstract nia).
+    Defined.
+
+   
+    Fixpoint pair_unzip {A : Type} {n : nat} : 
+      Vector.t (Vector.t A 2) n -> Vector.t A (2 * n).
+    Proof.
+      intros v.
+      refine
+        (match v in Vector.t _ n' return Vector.t _ (2 * n')  
+        with 
+        | [] => []
+        | Vector.cons _ vh nt vt => _ 
+        end).
+        replace (2 * S nt) with  (2 + 2 * nt); try (abstract nia).
+        exact (vh ++ pair_unzip _ _ vt).
+    Defined.
+      
+
+
+End Util.
+
 
 (* Discrete Logarithm Zero Knowlege Proof *) 
 Section DL. 
@@ -64,56 +168,9 @@ Section DL.
     Section Def. 
 
 
-        (*
-          g₁ h₁ x₁ gs hs xs us c
-          Proves that x₁ is not equal to any element in xs, i.e.,
-          ∀ x : F, In x xs -> x <> x₁
-          using Okamoto protocol
-        *)
-        (* don't reuse the random numbers! *)
-        (* can I use the same challenge? *)
+       
 
-        Definition generalised_construct_neq_conversations_okamoto :
-          ∀ {n : nat}, F -> G -> G ->     
-          Vector.t F (1 + n) ->
-          Vector.t G (1 + n) -> Vector.t G (1 + n) -> 
-          Vector.t F  (2 * (1 + n)) -> F -> 
-          @sigma_proto F G (1 + n) 1 (2 * (1 + n)).
-        Proof.
-          refine(fix Fn n {struct n} := 
-            match n with 
-            | 0 => fun  x₁ g₁ h₁ xs gs hs  us c => _
-            | S n' => fun  x₁ g₁ h₁  xs gs hs  us c => _ 
-            end); cbn in * |- *.
-          +
-            (* base case *)
-            destruct (vector_inv_S xs) as (x₂ & _).
-            destruct (vector_inv_S gs) as (g₂ & _).
-            destruct (vector_inv_S hs) as (h₂ & _).
-            destruct (vector_inv_S us) as (u₁ & ustl & _).
-            destruct (vector_inv_S ustl) as (u₂ & _).
-            exact ([gop ((gop g₁ g₂)^u₁) ((gop h₁ h₂)^u₂)]; [c];
-              [u₁ + c * x₁ * inv (x₁ - x₂); u₂ + c * inv (x₂ - x₁)]).
-          +
-            (* induction case *)
-            destruct (vector_inv_S gs) as (g₂ & gstl & _).
-            destruct (vector_inv_S hs) as (h₂ & hstl & _).
-            destruct (vector_inv_S xs) as (x₂ & xstl & _).
-            destruct (vector_inv_S us) as (u₁ & ustl & _).
-            destruct (vector_inv_S ustl) as (u₂ & ustll & _).
-            refine 
-              match (Fn _ x₁ g₁ h₁  xstl gstl hstl  
-                (@subst_vector F _ _ ustll (eq_sym (nat_succ_eq n' (n' + 0)))) c)
-              with 
-              | (a; _ ; r) => ([gop ((gop g₁ g₂)^u₁) ((gop h₁ h₂)^u₂)] ++ a; [c]; 
-                [u₁ + c * x₁ * inv (x₁ - x₂); u₂ + c * inv (x₂ - x₁)] ++ 
-                (@eq_rect nat (S (n' + S (n' + 0)))
-                  (fun x => Vector.t F x) r _  (nat_succ_eq n' (n' + 0))))
-              end.
-        Defined.
-
-
-        (* 
+       (* 
           xs : secrets 
           gs  hs : public values such h := g^x 
           us: randomness 
@@ -127,332 +184,119 @@ Section DL.
           (2 * (1 + n) + 2 * n + ...... + 2 = 
           (1 + n) (2 + n)
 
-          The amount of randomenss I need is : (1 + n) * (2 + n)
-        *)
-        (* 
-          This function is going to call 
-          generalised_construct_neq_conversations_okamoto
-          for each pair 
+          The amount of randomenss I need is : ((2 + n) + ((2 + n) * (1 + n)))
         *)
         
-        #[local]
-        Definition generalised_construct_neq_conversations_schnorr_supplement :
-          ∀ {n : nat}, Vector.t F (2 + n) -> 
-          Vector.t G (2 + n) -> 
-          Vector.t G (2 + n) ->  
-          Vector.t F ((2 + n) * (1 + n))-> F -> 
-          @sigma_proto F G (Nat.div ((2 + n) * (1 + n)) 2) 1 ((2 + n) * (1 + n)).
+
+       
+        Definition generalised_construct_neq_commitment {n : nat} : 
+          Vector.t G (2 + n) -> Vector.t G (2 + n) ->
+          Vector.t F ((2 + n) + ((2 + n) * (1 + n))) -> 
+          Vector.t G ((2 + n) + Nat.div ((2 + n) * (1 + n)) 2).
         Proof.
-          refine(fix Fn n {struct n} := 
-            match n with 
-            | 0 => fun xs gs hs us c => _
-            | S n' => fun xs gs hs us c => _ 
-            end); cbn in * |- *.
-          +
-            (* call Okamoto construction *)
-            refine 
-              (generalised_construct_neq_conversations_okamoto 
-              (hd xs) (hd gs) (hd hs) (tl xs) (tl gs) (tl hs) us c).
-          +
-            (* requires some complicated reasoning about arithmatic *)
-            (* inductive case *)
-            (* massage the goal *)
-            replace (S (S (n' + S (S (n' + S (S (n' + n' * S (S n')))))))) 
-            with ((2 * (2 + n')) + (S (n' + S (n' + n' * S n'))))%nat in us.
-             (* Take 2 * (S (S n')) from us *)
-            destruct (splitat (2 * (1 + S n')) us) as (usl & usr).
-            refine
-              match (generalised_construct_neq_conversations_okamoto 
-              (hd xs) (hd gs) (hd hs) (tl xs) (tl gs) (tl hs) usl c)
-              with
-              |(a₁; _; r₁) => _ 
-              end.
-            refine 
-              match Fn _ (tl xs) (tl gs) (tl hs)  usr c
-              with 
-              |(a₂; _; r₂) => _ 
-              end.
-            set (r := r₁ ++ r₂);
-            clearbody r.
-            set (a := a₁ ++ a₂);
-            clearbody a.
-            (* massage a *)
-            replace ((1 + S n' + fst (Nat.divmod (n' + S (n' + n' * S n')) 1 0 0)))%nat
-            with (fst (Nat.divmod (n' + S (S (n' + S (S (n' + n' * S (S n')))))) 1 1 1))
-            in a.
-            (* massage r *)
-            replace (2 * (1 + S n') + S (n' + S (n' + n' * S n')))%nat with 
-            (S (S (n' + S (S (n' + S (S (n' + n' * S (S n')))))))) in r.
-            refine (a; [c]; r).
-            all:try nia.
-            eapply nat_divmod.
+          intros gs hs us.
+          (* split the randomness us at 2 + n *)
+          destruct (splitat (2 + n) us) as (usl & usr).
+          (* usl for AND commitment and usr for Okamoto protocol *)
+          set (and_commit := @construct_and_conversations_schnorr_commitment
+            F G gpow _ gs usl).
+          (* construct gs pairs*)
+          set (gs_pairs := Vector.map (fun '(g₁, g₂) => gop g₁ g₂)
+            (generate_pairs_of_vector gs)).
+          set (hs_pairs := Vector.map (fun '(h₁, h₂) => gop h₁ h₂) 
+            (generate_pairs_of_vector hs)).
+          assert(ha : (2 * (Nat.div ((2 + n) * (1 + n)) 2) = 
+          ((2 + n) * (1 + n)))%nat). eapply nat_div_2.
+          replace (2 * Nat.div ((2 + n) * (1 + n)) 2)%nat with 
+          (Nat.div ((2 + n) * (1 + n)) 2 + Nat.div ((2 + n) * (1 + n)) 2)%nat in ha;
+          try (abstract nia).
+          rewrite <-ha in usr; clear ha.
+          destruct (splitat (Nat.div ((2 + n) * (1 + n)) 2) usr) as 
+          (usrl & usrr).
+          (* Okamoto commitment *)
+          set (oka_commitment := zip_with (fun '(gg, hh) '(u₁, u₂) =>
+            @okamoto_commitment F G gid gop gpow
+            [gg; hh] [u₁; u₂]) (zip_with pair gs_pairs hs_pairs)
+            (zip_with pair usrl usrr)).
+          refine(and_commit ++ oka_commitment).
         Defined.
 
+        
+        
+        Definition generalised_construct_neq_response {n : nat} : 
+          Vector.t F (2 + n) -> Vector.t F ((2 + n) + ((2 + n) * (1 + n))) -> 
+          F -> Vector.t F ((2 + n) + (2 + n) * (1 + n)).
+        Proof.
+          intros xs us c.
+          set (xs_pair := generate_pairs_of_vector xs).
+          (* split the randomness us at 2 + n *)
+          destruct (splitat (2 + n) us) as (usl & usr).
+          (* usl goes for AND response *)
+          set (and_response := @construct_and_conversations_schnorr_response
+            F add mul _ xs usl c).
+          assert(ha : (2 * (Nat.div ((2 + n) * (1 + n)) 2) = 
+          ((2 + n) * (1 + n)))%nat). eapply nat_div_2.
+          replace (2 * Nat.div ((2 + n) * (1 + n)) 2)%nat with 
+          (Nat.div ((2 + n) * (1 + n)) 2 + Nat.div ((2 + n) * (1 + n)) 2)%nat in ha;
+          try (abstract nia).
+          rewrite <-ha in usr; clear ha.
+          destruct (splitat (Nat.div ((2 + n) * (1 + n)) 2) usr) as 
+          (usrl & usrr).
+          (* Okamoto response *)
+          set (oka_response := pair_unzip (zip_with (fun '(x₁, x₂) '(u₁, u₂) => 
+              @okamoto_response F add mul [x₁ * inv (x₁ - x₂); inv (x₂ - x₁)]
+              [u₁; u₂] c) xs_pair (zip_with pair usrl usrr))).
+          rewrite nat_div_2 in oka_response.
+          exact (and_response ++ oka_response).
+        Defined.
 
         (* input xs, gs, hs, us, c *)
         (* size of proofs is O(n^2) for NEQ if 
           we have n statements.
         *) 
-        Definition generalised_construct_neq_conversations_schnorr {n : nat} : 
+        Definition generalised_construct_neq_conversations_real_transcript {n : nat} : 
           Vector.t F (2 + n) -> Vector.t G (2 + n) -> 
           Vector.t G (2 + n) -> 
           Vector.t F ((2 + n) + ((2 + n) * (1 + n))) -> F ->
           @sigma_proto F G ((2 + n) + Nat.div ((2 + n) * (1 + n)) 2) 1
             ((2 + n) + (2 + n) * (1 + n)).
         Proof.
-          (* first I compute AND protocol *)
           intros xs gs hs us c.
-          (* split the randomness us at 2 + n *)
-          destruct (splitat (2 + n) us) as (usl & usr).
-          (* Now run AND protocol *)
-          Print construct_and_conversations_schnorr.
-          (refine 
-            match @construct_and_conversations_schnorr F 
-            add mul G gpow _ xs gs usl c with 
-            | (a; _; r) => _ 
-            end).
-          (* Now call supplement protocol *)
-          (refine 
-            match generalised_construct_neq_conversations_schnorr_supplement 
-              xs gs hs usr c with 
-            | (a₁; _; r₁) => (a ++ a₁; [c]; r ++ r₁)
-            end).
-        Defined. 
-
-        (* simulator *)
-        (* Does not involve secret *)
-        (* g₁ h₁ gh hs us c *)
-        #[local]
-        Definition generalised_construct_neq_conversations_simulator_okamoto :
-          ∀ {n : nat}, G -> G ->
-          Vector.t G (1 + n) -> 
-          Vector.t G (1 + n) -> 
-          Vector.t F  (2 * (1 + n)) -> F -> 
-          @sigma_proto F G (1 + n) 1 (2 * (1 + n)).
-        Proof.
-          refine(fix Fn n {struct n} := 
-            match n with 
-            | 0 => fun g₁ h₁ gs hs us c => _
-            | S n' => fun g₁ h₁ gs hs us c => _ 
-            end); cbn in * |- *.
-          +
-            destruct (vector_inv_S gs) as (g₂ & _).
-            destruct (vector_inv_S hs) as (h₂ & _).
-            destruct (vector_inv_S us) as (u₁ & ustl & _).
-            destruct (vector_inv_S ustl) as (u₂ & _).
-            exact
-            ([gop ((gop g₁ g₂)^u₁) (gop ((gop h₁ h₂)^u₂) g₂^(opp c))]; [c];
-              [u₁; u₂]).
-          +
-            destruct (vector_inv_S gs) as (g₂ & gstl & _).
-            destruct (vector_inv_S hs) as (h₂ & hstl & _).
-            destruct (vector_inv_S us) as (u₁ & ustl & _).
-            destruct (vector_inv_S ustl) as (u₂ & ustll & _).
-            refine 
-              match Fn _ g₁ h₁ gstl hstl 
-                (@subst_vector F _ _ ustll (eq_sym (nat_succ_eq n' (n' + 0)))) c 
-              with 
-              | (a; _; r) => 
-                ([gop ((gop g₁ g₂)^u₁) (gop ((gop h₁ h₂)^u₂) g₂^(opp c))] ++ a; [c]; _)
-              end.
-            replace (S (n' + S (n' + 0)))%nat with 
-            (n' + S (S (n' + 0)))%nat in r.
-            exact ([u₁; u₂] ++ r).
-            nia.
+          exact (generalised_construct_neq_commitment gs hs us; [c];
+          generalised_construct_neq_response xs us c).
         Defined.
 
-        
-        (* gs hs us c *)
-        #[local]
-        Definition generalised_construct_neq_conversations_simulator_supplement :
-          ∀ {n : nat}, 
-          Vector.t G (2 + n) -> 
-          Vector.t G (2 + n) -> 
-          Vector.t F ((2 + n) * (1 + n)) -> F -> 
-          @sigma_proto F G (Nat.div ((2 + n) * (1 + n)) 2) 1 ((2 + n) * (1 + n)).
-        Proof.
-          refine(fix Fn n {struct n} := 
-            match n with 
-            | 0 => fun gs hs us c => _
-            | S n' => fun gs hs us c => _ 
-            end); cbn in * |- *.
-          +
-            exact (generalised_construct_neq_conversations_simulator_okamoto
-            (hd gs) (hd hs) (tl gs) (tl hs) us c).
-          +
-            replace (S (S (n' + S (S (n' + S (S (n' + n' * S (S n')))))))) 
-            with ((2 * (2 + n')) + (S (n' + S (n' + n' * S n'))))%nat in us.
-             (* Take 2 * (S (S n')) from us *)
-            destruct (splitat (2 * (1 + S n')) us) as (usl & usr).
-            refine
-              match (generalised_construct_neq_conversations_simulator_okamoto 
-              (hd gs) (hd hs) (tl gs) (tl hs) usl c)
-              with
-              |(a₁; _; r₁) => _ 
-              end.
-            refine 
-              match Fn _ (tl gs) (tl hs) usr c
-              with 
-              |(a₂; _; r₂) => _ 
-              end.
-            set (r := r₁ ++ r₂);
-            clearbody r.
-            set (a := a₁ ++ a₂);
-            clearbody a.
-            replace ((1 + S n' + fst (Nat.divmod (n' + S (n' + n' * S n')) 1 0 0)))%nat
-            with (fst (Nat.divmod (n' + S (S (n' + S (S (n' + n' * S (S n')))))) 1 1 1))
-            in a.
-            (* massage r *)
-            replace (2 * (1 + S n') + S (n' + S (n' + n' * S n')))%nat with 
-            (S (S (n' + S (S (n' + S (S (n' + n' * S (S n')))))))) in r.
-            refine (a; [c]; r).
-            all:try nia.
-            eapply nat_divmod.
-        Defined.
-
-
-            
-        (* input gs, hs, us, c *)
-        (* does not involve secret *)
-        Definition generalised_construct_neq_conversations_simulator {n : nat} : 
-          Vector.t G (2 + n) -> Vector.t G (2 + n) -> 
+        Definition generalised_construct_neq_conversations_simulator_transcript 
+          {n : nat} : Vector.t G (2 + n) -> Vector.t G (2 + n) -> 
           Vector.t F ((2 + n) + ((2 + n) * (1 + n))) -> F ->
           @sigma_proto F G ((2 + n) + Nat.div ((2 + n) * (1 + n)) 2) 1
             ((2 + n) + (2 + n) * (1 + n)).
         Proof.
-          (* first I compute AND protocol simulator *)
           intros gs hs us c.
-          (* split the randomness us at 2 + n *)
           destruct (splitat (2 + n) us) as (usl & usr).
-          (* run AND protocol simulator *)
-          refine 
-            match @construct_and_conversations_simulator F 
-            opp G gop gpow _ gs hs usl c with 
-            | (a; _; r) => _ 
-            end.
-          refine 
-            match generalised_construct_neq_conversations_simulator_supplement 
-              gs hs usr c with 
-            | (a₁; _; r₁) => (a ++ a₁; [c]; r ++ r₁)
-            end.
+          (* AND simulator commitment *)
+          set (and_sim_comm := 
+            @construct_and_conversations_simulator_commitment
+            F opp G gop gpow _ gs hs usl c).
+          assert(ha : (2 * (Nat.div ((2 + n) * (1 + n)) 2) = 
+          ((2 + n) * (1 + n)))%nat). eapply nat_div_2.
+          replace (2 * Nat.div ((2 + n) * (1 + n)) 2)%nat with 
+          (Nat.div ((2 + n) * (1 + n)) 2 + Nat.div ((2 + n) * (1 + n)) 2)%nat in ha;
+          try (abstract nia).
+          rewrite <-ha in usr; clear ha.
+          destruct (splitat (Nat.div ((2 + n) * (1 + n)) 2) usr) as 
+          (usrl & usrr).
+          set (oka_sim_comm := zip_with (fun '((g₁, g₂), (h₁, h₂)) '(u₁, u₂) =>
+            @okamoto_simulator_protocol_commitment F opp G gid gop gpow 
+              [gop g₁ g₂; gop h₁ h₂] g₂ [u₁; u₂] c)
+              (zip_with pair 
+                (generate_pairs_of_vector gs) 
+                (generate_pairs_of_vector hs))
+              (zip_with pair usrl usrr)).
+          refine (and_sim_comm ++ oka_sim_comm; [c]; us).
         Defined.
 
-        (* end simulator *)
-
-        (* verification equation *)
-
-        (* verification equation of Okamoto protocol *)
-        (* g₁ h₁ gs hs sigma_proof *)
-        #[local]
-        Definition generalised_neq_accepting_conversations_okamoto :
-          ∀ {n : nat}, G -> G ->    
-          Vector.t G (1 + n) -> Vector.t G (1 + n) -> 
-          @sigma_proto F G (1 + n) 1 (2 * (1 + n)) -> bool.
-        Proof.
-          refine(fix Fn n {struct n} := 
-            match n with 
-            | 0 => fun  g₁ h₁ gs hs us => _
-            | S n' => fun  g₁ h₁ gs hs us => _ 
-            end); cbn in * |- *.
-          +
-            refine 
-              match us with 
-              |(a; c; r) => _ 
-              end.
-            (*
-              Verifies the following equation
-              (g₁ * g₂)^r₁ * (h₁ * h₂)^r₂ = a₁ * g₂^c₁
-            *)
-            destruct (vector_inv_S gs) as (g₂ & _).
-            destruct (vector_inv_S hs) as (h₂ & _).
-            destruct (vector_inv_S a) as (a₁ & _).
-            destruct (vector_inv_S c) as (c₁ & _).
-            destruct (vector_inv_S r) as (r₁ & rtl & _).
-            destruct (vector_inv_S rtl) as (r₂ & _).
-            refine 
-              match Gdec 
-                (gop ((gop g₁ g₂)^r₁) ((gop h₁ h₂)^r₂)) 
-                (gop a₁ (g₂^c₁))
-              with 
-              | left _ => true 
-              | right _ => false 
-              end.
-          +
-            refine 
-              match us with 
-              |(a; c; r) => _ 
-              end.
-            destruct (vector_inv_S gs) as (g₂ & gstl & _).
-            destruct (vector_inv_S hs) as (h₂ & hstl & _).
-            destruct (vector_inv_S a) as (a₁ & atl & _).
-            destruct (vector_inv_S c) as (c₁ & _).
-            destruct (vector_inv_S r) as (r₁ & rtl & _).
-            destruct (vector_inv_S rtl) as (r₂ & rtll & _).
-            refine 
-              match Gdec 
-                (gop ((gop g₁ g₂)^r₁) ((gop h₁ h₂)^r₂)) 
-                (gop a₁ (g₂^c₁))
-              with
-              | left _ => Fn _ g₁ h₁ gstl hstl (atl; c; _) (* check the rest *)
-              | right _ => false (* no point of checking the rest *)
-              end.
-            (* 
-              massage rtll to the goal
-            *)
-            refine 
-              (@eq_rect nat (n' + S (S (n' + 0)))%nat 
-                (fun x => Vector.t F x) rtll (S (n' + S (n' + 0)))
-                (eq_sym (nat_succ_eq n' (n' + 0)))).
-        Defined.
-
-        
-        Definition generalised_neq_accepting_conversations_supplement :
-          forall {n : nat}, 
-          Vector.t G (2 + n) -> Vector.t G (2 + n) ->
-          @sigma_proto F G (Nat.div ((2 + n) * (1 + n)) 2) 1
-            ((2 + n) * (1 + n)) -> bool.
-        Proof.
-          refine(fix Fn n {struct n} := 
-            match n with 
-            | 0 => fun gs hs sig => _
-            | S n' => fun gs hs sig => _ 
-            end); cbn in * |- *.
-          +
-            (* call Okamoto verification *)
-            refine 
-              (generalised_neq_accepting_conversations_okamoto 
-                (hd gs) (hd hs) (tl gs) (tl hs) sig).
-          +
-            (* inductive case *)
-            refine 
-              match sig with 
-              |(a; c; r) => _ 
-              end.
-            destruct (vector_inv_S gs) as (g₁ & gstl & _).
-            destruct (vector_inv_S hs) as (h₁ & hstl & _).
-            rewrite nat_divmod in a.
-            destruct (splitat (2 + n') a) as (al & ar).
-            replace (S (S (n' + S (S (n' + S (S (n' + n' * S (S n')))))))) 
-            with ((2 * (2 + n')) + (S (n' + S (n' + n' * S n'))))%nat in r.
-            destruct (splitat (2 * (2 + n')) r) as (rl & rr).
-            (* 
-              Call generalised_neq_conversations_okamoto and if it 
-              returns true than continue checking else 
-              break. 
-            *)
-            refine 
-              match generalised_neq_accepting_conversations_okamoto 
-                g₁ h₁ gstl hstl (al; c; rl)
-              with 
-              | true => Fn _ gstl hstl (ar ; c; rr)
-              | _ => false
-              end.
-            nia.
-        Defined.
-
-
-
-
+        (* verification *)
         Definition generalised_neq_accepting_conversations {n : nat} :
           Vector.t G (2 + n) -> Vector.t G (2 + n) ->
           @sigma_proto F G ((2 + n) + Nat.div ((2 + n) * (1 + n)) 2) 1
@@ -471,16 +315,20 @@ Section DL.
           (* Run AND verifier on (al; c; rl) *)
           refine 
             match 
-              @generalised_and_accepting_conversations F G gop gpow Gdec _ gs hs (al; c; rl)
+              @generalised_and_accepting_conversations F G gop gpow Gdec _ 
+              gs hs (al; c; rl)
             with 
             | true => _ 
             | _ => false (* No point of checking futher *) 
             end.
           (* run Okamoto verifier on (ar; c; rr) *)
-          exact (generalised_neq_accepting_conversations_supplement gs hs (ar; c; rr)).
-        Defined.
-          
-        (* end verification *)
+          set (gs_pairs := Vector.map (fun '(g₁, g₂) => gop g₁ g₂)
+            (generate_pairs_of_vector gs)).
+          set (hs_pairs := Vector.map (fun '(h₁, h₂) => gop h₁ h₂) 
+            (generate_pairs_of_vector hs)).
+
+
+        Admitted.
 
         (* distribution (zero-knowledge) *)
 
@@ -492,7 +340,7 @@ Section DL.
           (* draw ((2 + n) + ((1 + n) + (1 + n))) random elements *)
           us <- repeat_dist_ntimes_vector 
             (uniform_with_replacement lf Hlfn) ((2 + n) + ((2 + n) * (1 + n))) ;;
-          Ret (generalised_construct_neq_conversations_schnorr xs gs hs us c).
+          Ret (generalised_construct_neq_conversations_real_transcript xs gs hs us c).
 
 
         Definition generalised_neq_simulator_distribution  
@@ -503,18 +351,12 @@ Section DL.
           (* draw ((2 + n) + ((1 + n) + (1 + n))) random elements *)
           us <- repeat_dist_ntimes_vector 
             (uniform_with_replacement lf Hlfn) ((2 + n) + ((2 + n) * (1 + n))) ;;
-          Ret (generalised_construct_neq_conversations_simulator gs hs us c).
-        
+          Ret (generalised_construct_neq_conversations_simulator_transcript gs hs us c).
+
     End Def. 
 
-    Section Proofs.
-      
-      
-      
-
-
-
-    End Proofs.
+    Section Proofs. 
+    
+    End Proofs. 
   End Neq.
 End DL.
-*)
